Better arrays of constant-size elements, explicit precondition

examples/lowparse/LowParse.Spec.Array.fst
@@ -5,13 +5,21 @@ include LowParse.Spec.Seq
 module Seq = FStar.Seq
 module PL = LowParse.Spec.List
 
+module U32 = FStar.UInt32
+
 type array (t: Type) (n: nat) = (s: Seq.seq t { Seq.length s == n } )
 
-let array_type_of_parser_kind_precond (elem_byte_size: nat) (array_byte_size: nat) : GTot bool =
-  elem_byte_size > 0 &&
+let array_type_of_parser_kind_precond
+  (#elem_byte_size: nat)
+  (#k: constant_size_parser_kind)
+  (#t: Type0)
+  (p: parser (ParserStrong (StrongConstantSize elem_byte_size k)) t)
+  (array_byte_size: nat)
+: GTot bool
+= elem_byte_size > 0 &&
   array_byte_size % elem_byte_size = 0
 
-let array_type_of_parser
+let array_type_of_parser'
   (#elem_byte_size: nat)
   (#k: constant_size_parser_kind)
   (#t: Type0)
@@ -19,7 +27,7 @@ let array_type_of_parser
   (array_byte_size: nat)
 : Pure Type0
   (requires (
-    array_type_of_parser_kind_precond elem_byte_size array_byte_size
+    array_type_of_parser_kind_precond p array_byte_size
   ))
   (ensures (fun _ -> True))
 = array t (array_byte_size / elem_byte_size)
@@ -33,11 +41,11 @@ val parse_array_correct
   (b: bytes32)
 : Lemma
   (requires (
-    array_type_of_parser_kind_precond elem_byte_size array_byte_size /\
+    array_type_of_parser_kind_precond p array_byte_size /\
     Some? (parse (parse_flbytes (parse_seq p) array_byte_size) b)
   ))
   (ensures (
-    array_type_of_parser_kind_precond elem_byte_size array_byte_size /\ (
+    array_type_of_parser_kind_precond p array_byte_size /\ (
     let pb = parse (parse_flbytes (parse_seq p) array_byte_size) b in
     Some? pb /\ (
     let (Some (data, _)) = pb in
@@ -57,8 +65,8 @@ let parse_array'
   (#t: Type0)
   (p: parser (ParserStrong (StrongConstantSize elem_byte_size k)) t)
   (array_byte_size: nat)
-  (precond: squash (array_type_of_parser_kind_precond elem_byte_size array_byte_size))
-: Tot (bare_parser (array_type_of_parser p array_byte_size))
+  (precond: squash (array_type_of_parser_kind_precond p array_byte_size))
+: Tot (bare_parser (array_type_of_parser' p array_byte_size))
 = fun (b: bytes32) ->
   match parse (parse_flbytes (parse_seq p) array_byte_size) b with
   | None -> None
@@ -73,10 +81,10 @@ let parse_array_injective
   (#t: Type0)
   (p: parser (ParserStrong (StrongConstantSize elem_byte_size k)) t)
   (array_byte_size: nat)
-  (precond: squash (array_type_of_parser_kind_precond elem_byte_size array_byte_size))
+  (precond: squash (array_type_of_parser_kind_precond p array_byte_size))
 : Lemma
   (injective (parse_array' p array_byte_size precond))
-= let p' : bare_parser (array_type_of_parser p array_byte_size) = parse_array' p array_byte_size precond in
+= let p' : bare_parser (array_type_of_parser' p array_byte_size) = parse_array' p array_byte_size precond in
   let prf
     (b1 b2: bytes32)
   : Lemma
@@ -100,13 +108,15 @@ val parse_total_constant_size_elem_parse_list_total
   (b: bytes32)
 : Lemma
   (requires (
-    array_type_of_parser_kind_precond elem_byte_size array_byte_size /\
+    array_type_of_parser_kind_precond p array_byte_size /\
     Seq.length b % elem_byte_size == 0
   ))
   (ensures (
     Some? (parse (PL.parse_list p) b)
   ))
   (decreases (Seq.length b))
+
+#set-options "--z3rlimit 128"
 
 let rec parse_total_constant_size_elem_parse_list_total #elem_byte_size #t p array_byte_size b =
   if Seq.length b = 0
@@ -120,15 +130,17 @@ let rec parse_total_constant_size_elem_parse_list_total #elem_byte_size #t p arr
     let b' = Seq.slice b consumed (Seq.length b) in
     FStar.Math.Lemmas.lemma_mod_plus (Seq.length b') 1 elem_byte_size;
     parse_total_constant_size_elem_parse_list_total p array_byte_size b' ;    
-    assume (Some? (parse (PL.parse_list p) b))
+    assert (Some? (parse (PL.parse_list p) b))
   end
+
+#reset-options
 
 val parse_total_constant_size_elem_parse_array_total'
   (#elem_byte_size: nat)
   (#t: Type0)
   (p: parser (ParserStrong (StrongConstantSize elem_byte_size ConstantSizeTotal)) t)
   (array_byte_size: nat)
-  (precond: squash (array_type_of_parser_kind_precond elem_byte_size array_byte_size))
+  (precond: squash (array_type_of_parser_kind_precond p array_byte_size))
   (b: bytes32)
 : Lemma
   (requires (
@@ -149,7 +161,7 @@ let parse_total_constant_size_elem_parse_array_total
   (#t: Type0)
   (p: parser (ParserStrong (StrongConstantSize elem_byte_size k)) t)
   (array_byte_size: nat)
-  (precond: squash (array_type_of_parser_kind_precond elem_byte_size array_byte_size))
+  (precond: squash (array_type_of_parser_kind_precond p array_byte_size))
 : Lemma
   (ensures (
     ConstantSizeTotal? k ==> (forall (b: bytes32) .
@@ -162,14 +174,298 @@ let parse_total_constant_size_elem_parse_array_total
     Classical.forall_intro (Classical.move_requires (parse_total_constant_size_elem_parse_array_total' p' array_byte_size ()))
   else ()
 
-let parse_array
+abstract
+let parse_array_precond
   (#elem_byte_size: nat)
   (#k: constant_size_parser_kind)
   (#t: Type0)
   (p: parser (ParserStrong (StrongConstantSize elem_byte_size k)) t)
-  (array_byte_size: nat)
-  (precond: squash (array_type_of_parser_kind_precond elem_byte_size array_byte_size))
-: Tot (parser (ParserStrong (StrongConstantSize array_byte_size k)) (array_type_of_parser p array_byte_size))
-= parse_array_injective p array_byte_size precond;
-  parse_total_constant_size_elem_parse_array_total p array_byte_size precond;
-  parse_array' p array_byte_size precond
+  (array_byte_size: U32.t)
+: Tot Type0
+= unit -> Lemma
+  (array_type_of_parser_kind_precond p (U32.v array_byte_size))
+
+abstract
+let parse_array_precond_intro
+  (#elem_byte_size: nat)
+  (#k: constant_size_parser_kind)
+  (#t: Type0)
+  (p: parser (ParserStrong (StrongConstantSize elem_byte_size k)) t)
+  (array_byte_size: U32.t)
+  (x: (
+    unit -> Lemma
+    (array_type_of_parser_kind_precond p (U32.v array_byte_size))
+  ))
+: Tot (parse_array_precond p array_byte_size)
+= x
+
+abstract
+let parse_array_precond_elim
+  (#elem_byte_size: nat)
+  (#k: constant_size_parser_kind)
+  (#t: Type0)
+  (#p: parser (ParserStrong (StrongConstantSize elem_byte_size k)) t)
+  (#array_byte_size: U32.t)
+  (x: parse_array_precond p array_byte_size)
+: Lemma
+  (array_type_of_parser_kind_precond p (U32.v array_byte_size))
+= x ()
+
+let array_type_of_parser
+  (#elem_byte_size: nat)
+  (#k: constant_size_parser_kind)
+  (#t: Type0)
+  (#p: parser (ParserStrong (StrongConstantSize elem_byte_size k)) t)
+  (#array_byte_size: U32.t)
+  (precond: parse_array_precond p array_byte_size)
+: Tot Type0
+= parse_array_precond_elim precond;
+  array_type_of_parser' p (U32.v array_byte_size)
+
+#set-options "--z3rlimit 32"
+
+let parse_array
+  (#elem_byte_size: nat)
+  (#k: constant_size_parser_kind)
+  (#t: Type0)
+  (#p: parser (ParserStrong (StrongConstantSize elem_byte_size k)) t)
+  (#array_byte_size: U32.t)
+  (precond: parse_array_precond p array_byte_size)
+: Tot (parser (ParserStrong (StrongConstantSize (U32.v array_byte_size) k)) (array_type_of_parser precond))
+= parse_array_precond_elim precond;
+  parse_array_injective p (U32.v array_byte_size) ();
+  parse_total_constant_size_elem_parse_array_total p (U32.v array_byte_size) ();
+  parse_array' p (U32.v array_byte_size) ()
+
+#reset-options
+
+include LowParse.Spec.VLBytes
+
+type vlarray (t: Type) (min max: nat) =
+  (s: Seq.seq t {
+    let l = Seq.length s in
+    min <= l /\ l <= max
+  })
+
+let vlarray_type_of_parser_kind_precond'
+  (#elem_byte_size: nat)
+  (#k: constant_size_parser_kind)
+  (#t: Type0)
+  (p: parser (ParserStrong (StrongConstantSize elem_byte_size k)) t)
+  (array_byte_size_min array_byte_size_max: nat) : GTot bool =
+  elem_byte_size > 0 &&
+  array_byte_size_min % elem_byte_size = 0 &&
+  array_byte_size_max % elem_byte_size = 0 &&
+  array_byte_size_max > 0
+
+let vlarray_type_of_parser_kind_precond
+  (#elem_byte_size: nat)
+  (#k: constant_size_parser_kind)
+  (#t: Type0)
+  (p: parser (ParserStrong (StrongConstantSize elem_byte_size k)) t)
+  (array_byte_size_min array_byte_size_max: U32.t) : GTot bool =
+  vlarray_type_of_parser_kind_precond' p (U32.v array_byte_size_min) (U32.v array_byte_size_max)
+
+let vlarray_type_of_parser'
+  (#elem_byte_size: nat)
+  (#k: constant_size_parser_kind)
+  (#t: Type0)
+  (p: parser (ParserStrong (StrongConstantSize elem_byte_size k)) t)
+  (array_byte_size_min array_byte_size_max: U32.t)
+: Pure Type0
+  (requires (
+    vlarray_type_of_parser_kind_precond p array_byte_size_min array_byte_size_max
+  ))
+  (ensures (fun _ -> True))
+= vlarray t (U32.v array_byte_size_min / elem_byte_size) (U32.v array_byte_size_max / elem_byte_size)
+
+val parse_vlarray_correct
+  (#elem_byte_size: nat)
+  (#k: constant_size_parser_kind)
+  (#t: Type0)
+  (p: parser (ParserStrong (StrongConstantSize elem_byte_size k)) t)
+  (array_byte_size_min array_byte_size_max: U32.t)
+  (b: bytes32)
+: Lemma
+  (requires (
+    vlarray_type_of_parser_kind_precond p array_byte_size_min array_byte_size_max /\
+    Some? (parse (parse_bounded_vlbytes array_byte_size_min array_byte_size_max (parse_seq p)) b)
+  ))
+  (ensures (
+    vlarray_type_of_parser_kind_precond p array_byte_size_min array_byte_size_max /\ (
+    let pb = parse (parse_bounded_vlbytes array_byte_size_min array_byte_size_max (parse_seq p)) b in
+    Some? pb /\ (
+    let (Some (data, _)) = pb in
+    let l = Seq.length data in
+    U32.v array_byte_size_min / elem_byte_size <= l /\
+    l <= U32.v array_byte_size_max / elem_byte_size
+  ))))
+
+#set-options "--z3rlimit 128"
+
+let parse_vlarray_correct #elem_byte_size #k #t p array_byte_size_min array_byte_size_max b =
+  let (Some (data, consumed)) = parse (parse_bounded_vlbytes array_byte_size_min array_byte_size_max (parse_seq p)) b in
+  let sz : integer_size = log256 array_byte_size_max in
+  assert (consumed >= sz);
+  let b' : bytes32 = Seq.slice b sz consumed in
+  assert (b' == Seq.slice (Seq.slice b sz (Seq.length b)) 0 (consumed - sz));
+  let (Some (data', consumed')) = parse (parse_seq p) b' in
+  assert (data == data');
+  assert ((consumed' <: nat) == consumed - sz);
+  seq_length_constant_size_parser_correct p b';
+  FStar.Math.Lemmas.multiple_division_lemma (Seq.length data) elem_byte_size;
+  FStar.Math.Lemmas.lemma_div_le (U32.v array_byte_size_min) consumed' elem_byte_size ;
+  FStar.Math.Lemmas.lemma_div_le consumed' (U32.v array_byte_size_max) elem_byte_size
+
+#reset-options
+
+#set-options "--z3rlimit 64"
+
+let parse_vlarray'
+  (#elem_byte_size: nat)
+  (#k: constant_size_parser_kind)
+  (#t: Type0)
+  (p: parser (ParserStrong (StrongConstantSize elem_byte_size k)) t)
+  (array_byte_size_min array_byte_size_max: U32.t)
+  (precond: squash (vlarray_type_of_parser_kind_precond p array_byte_size_min array_byte_size_max))
+: Tot (bare_parser (vlarray_type_of_parser' p array_byte_size_min array_byte_size_max))
+= fun (b: bytes32) ->
+  match parse (parse_bounded_vlbytes array_byte_size_min array_byte_size_max (parse_seq p)) b with
+  | None -> None
+  | Some (data, consumed) ->
+    parse_vlarray_correct p array_byte_size_min array_byte_size_max b;
+    let data' : vlarray t (U32.v array_byte_size_min / elem_byte_size) (U32.v array_byte_size_max / elem_byte_size) = data in
+    Some (data' , consumed)
+
+#reset-options
+
+let parse_vlarray_injective
+  (#elem_byte_size: nat)
+  (#k: constant_size_parser_kind)
+  (#t: Type0)
+  (p: parser (ParserStrong (StrongConstantSize elem_byte_size k)) t)
+  (array_byte_size_min array_byte_size_max: U32.t)
+  (precond: squash (vlarray_type_of_parser_kind_precond p array_byte_size_min array_byte_size_max))
+: Lemma
+  (injective (parse_vlarray' p array_byte_size_min array_byte_size_max precond))
+= let p' : bare_parser (vlarray_type_of_parser' p array_byte_size_min array_byte_size_max) = parse_vlarray' p array_byte_size_min array_byte_size_max precond in
+  let prf
+    (b1 b2: bytes32)
+  : Lemma
+    (requires (injective_precond p' b1 b2))
+    (ensures (injective_postcond p' b1 b2))
+  = assert (injective_postcond (parse_bounded_vlbytes array_byte_size_min array_byte_size_max (parse_seq p)) b1 b2)
+  in
+  let prf'
+    (b1 b2: bytes32)
+  : Lemma
+    (injective_precond p' b1 b2 ==> injective_postcond p' b1 b2)
+  = Classical.move_requires (prf b1) b2
+  in
+  Classical.forall_intro_2 prf'
+
+#set-options "--z3rlimit 32"
+
+let parse_vlarray_no_lookahead
+  (#elem_byte_size: nat)
+  (#k: constant_size_parser_kind)
+  (#t: Type0)
+  (p: parser (ParserStrong (StrongConstantSize elem_byte_size k)) t)
+  (array_byte_size_min array_byte_size_max: U32.t)
+  (precond: squash (vlarray_type_of_parser_kind_precond p array_byte_size_min array_byte_size_max))
+: Lemma
+  (no_lookahead (parse_vlarray' p array_byte_size_min array_byte_size_max precond))
+= let p' : bare_parser (vlarray_type_of_parser' p array_byte_size_min array_byte_size_max) = parse_vlarray' p array_byte_size_min array_byte_size_max precond in
+  let prf
+    (b1 b2: bytes32)
+  : Lemma
+    (requires (no_lookahead_on_precond p' b1 b2))
+    (ensures (no_lookahead_on_postcond p' b1 b2))
+  = assert (no_lookahead_on (parse_bounded_vlbytes array_byte_size_min array_byte_size_max (parse_seq p)) b1 b2)
+  in
+  let prf'
+    (b1 b2: bytes32)
+  : Lemma
+    (no_lookahead_on p' b1 b2)
+  = Classical.move_requires (prf b1) b2
+  in
+  Classical.forall_intro_2 prf'
+
+let parse_vlarray_no_lookahead_weak
+  (#elem_byte_size: nat)
+  (#k: constant_size_parser_kind)
+  (#t: Type0)
+  (p: parser (ParserStrong (StrongConstantSize elem_byte_size k)) t)
+  (array_byte_size_min array_byte_size_max: U32.t)
+  (precond: squash (vlarray_type_of_parser_kind_precond p array_byte_size_min array_byte_size_max))
+: Lemma
+  (no_lookahead_weak (parse_vlarray' p array_byte_size_min array_byte_size_max precond))
+= let p' : bare_parser (vlarray_type_of_parser' p array_byte_size_min array_byte_size_max) = parse_vlarray' p array_byte_size_min array_byte_size_max precond in
+  let prf
+    (b1 b2: bytes32)
+  : Lemma
+    (no_lookahead_weak_on p' b1 b2)
+  = assert (no_lookahead_weak_on (parse_bounded_vlbytes array_byte_size_min array_byte_size_max (parse_seq p)) b1 b2)
+  in
+  Classical.forall_intro_2 prf
+
+abstract
+let parse_vlarray_precond
+  (#elem_byte_size: nat)
+  (#k: constant_size_parser_kind)
+  (#t: Type0)
+  (p: parser (ParserStrong (StrongConstantSize elem_byte_size k)) t)
+  (array_byte_size_min array_byte_size_max: U32.t)
+: Tot Type0
+= unit -> Lemma
+  (vlarray_type_of_parser_kind_precond p array_byte_size_min array_byte_size_max)
+
+abstract
+let parse_vlarray_precond_intro
+  (#elem_byte_size: nat)
+  (#k: constant_size_parser_kind)
+  (#t: Type0)
+  (p: parser (ParserStrong (StrongConstantSize elem_byte_size k)) t)
+  (array_byte_size_min array_byte_size_max: U32.t)
+  (x: (unit -> Lemma
+    (vlarray_type_of_parser_kind_precond p array_byte_size_min array_byte_size_max)
+  ))
+: Tot (parse_vlarray_precond p array_byte_size_min array_byte_size_max)
+= x
+
+abstract
+let parse_vlarray_precond_elim
+  (#elem_byte_size: nat)
+  (#k: constant_size_parser_kind)
+  (#t: Type0)
+  (#p: parser (ParserStrong (StrongConstantSize elem_byte_size k)) t)
+  (#array_byte_size_min #array_byte_size_max: U32.t)
+  (x: parse_vlarray_precond p array_byte_size_min array_byte_size_max)
+: Lemma
+  (vlarray_type_of_parser_kind_precond p array_byte_size_min array_byte_size_max)
+= x ()
+
+let vlarray_type_of_parser
+  (#elem_byte_size: nat)
+  (#k: constant_size_parser_kind)
+  (#t: Type0)
+  (#p: parser (ParserStrong (StrongConstantSize elem_byte_size k)) t)
+  (#array_byte_size_min #array_byte_size_max: U32.t)
+  (precond: parse_vlarray_precond p array_byte_size_min array_byte_size_max)
+: Tot Type0
+= parse_vlarray_precond_elim precond;
+  vlarray_type_of_parser' p array_byte_size_min array_byte_size_max
+
+let parse_vlarray
+  (#elem_byte_size: nat)
+  (#k: constant_size_parser_kind)
+  (#t: Type0)
+  (#p: parser (ParserStrong (StrongConstantSize elem_byte_size k)) t)
+  (#array_byte_size_min #array_byte_size_max: U32.t)
+  (precond: parse_vlarray_precond p array_byte_size_min array_byte_size_max)
+: Tot (parser (ParserStrong StrongUnknown) (vlarray_type_of_parser precond))
+= parse_vlarray_precond_elim precond;
+  parse_vlarray_injective p array_byte_size_min array_byte_size_max ();
+  parse_vlarray_no_lookahead_weak p array_byte_size_min array_byte_size_max ();
+  parse_vlarray_no_lookahead p array_byte_size_min array_byte_size_max ();
+  parse_vlarray' p array_byte_size_min array_byte_size_max ()
